FoC/Computability/Compiler/Core/EncodedRewriters/ClosedConfigRunner/Simulator/PaddedEmitter/TerminalCore/Contracts.lean
@@ -1,4 +1,5 @@
 import FoC.Computability.Compiler.Core.EncodedRewriters.ClosedConfigRunner.Simulator.PaddedEmitter.TerminalCore.Core
+import FoC.Computability.Compiler.Core.EncodedRewriters.ClosedConfigRunner.Simulator.PaddedParser.Return
 
 set_option doc.verso true
 
